Edmonds_Blossom_Algorithm/Matching_Contraction_Expansion.thy
@@ -1,0 +1,893 @@
+theory Matching_Contraction_Expansion
+  imports Graph_Quotient Basic_Matching.Matching_Augmentation_Executable
+begin  
+
+locale blossom_matching_spec =
+  fixes empty_matching::'matching
+   and matching_invar::"'v set set \<Rightarrow> 'matching \<Rightarrow> bool"
+   and get_partner::"'matching \<Rightarrow> 'v \<Rightarrow> 'v"
+   and augment::"'matching \<Rightarrow> 'v list \<Rightarrow> 'matching"
+   and matching_abstract::"'matching \<Rightarrow> 'v set set"
+   and contract_path_at_matched::"'matching \<Rightarrow> 'v list \<Rightarrow> 'v \<Rightarrow> 'matching"
+   and expand_path_at_matched::"'matching \<Rightarrow> 'v list \<Rightarrow> 'v \<Rightarrow>'v \<Rightarrow> 'matching"
+   and add_alternatingly::"'matching \<Rightarrow> 'v list \<Rightarrow> 'matching"
+begin
+definition "contract_path_at_matched_precond G M p new_vert contr = 
+            (matching_invar G M \<and> hd p \<in> Vs (matching_abstract M) \<and>
+             alt_path (matching_abstract M) p \<and>  odd (length p) \<and>
+            distinct p \<and> new_vert \<notin>  Vs (matching_abstract M) - set p \<and>
+            contr = (\<lambda> x. if x \<in> set p then new_vert else x))"
+
+lemma contract_path_at_matched_precondE:
+  "\<lbrakk>contract_path_at_matched_precond G M p new_vert contr;
+    \<lbrakk>matching_invar G M; hd p \<in> Vs (matching_abstract M);
+    alt_path (matching_abstract M) p;  odd (length p);
+    distinct p; new_vert \<notin>  Vs (matching_abstract M) - set p;
+    contr = (\<lambda> x. if x \<in> set p then new_vert else x)\<rbrakk> \<Longrightarrow> P\<rbrakk>
+    \<Longrightarrow> P"
+and contract_path_at_matched_precondI:
+  "\<lbrakk>matching_invar G M; hd p \<in> Vs (matching_abstract M);
+    alt_path (matching_abstract M) p;  odd (length p);
+    distinct p; new_vert \<notin>  Vs (matching_abstract M) - set p;
+    contr = (\<lambda> x. if x \<in> set p then new_vert else x)\<rbrakk>
+    \<Longrightarrow> contract_path_at_matched_precond G M p new_vert contr"
+  by(auto simp add: contract_path_at_matched_precond_def)
+
+definition "expand_path_at_matched_precond G M old_vert mo new_vert p=
+      (matching_invar G M \<and> {old_vert, mo} \<in> matching_abstract M \<and> 
+       new_vert \<notin> Vs (matching_abstract M) - {old_vert} \<and> new_vert \<notin> set p \<and> 
+       set p \<inter> Vs (matching_abstract M) = {} \<and> even (length p) \<and> distinct p)"
+
+lemma expand_path_at_matched_precondE:
+  "\<lbrakk>expand_path_at_matched_precond G M old_vert mo new_vert p;
+    \<lbrakk>matching_invar G M; {old_vert, mo} \<in> matching_abstract M;
+     new_vert \<notin> Vs (matching_abstract M) - {old_vert}; new_vert \<notin> set p;
+       set p \<inter> Vs (matching_abstract M) = {}; even (length p); distinct p\<rbrakk> \<Longrightarrow> P\<rbrakk>
+   \<Longrightarrow> P"
+and expand_path_at_matched_precondD:
+  "\<lbrakk>matching_invar G M; {old_vert, mo} \<in> matching_abstract M;
+     new_vert \<notin> Vs (matching_abstract M) - {old_vert}; new_vert \<notin> set p;
+       set p \<inter> Vs (matching_abstract M) = {}; even (length p); distinct p\<rbrakk> 
+   \<Longrightarrow> expand_path_at_matched_precond G M old_vert mo new_vert p"
+  by(auto simp add: expand_path_at_matched_precond_def)
+
+definition "add_alternatingly_precond G M p = 
+            (matching_invar G M \<and> set p \<inter> Vs (matching_abstract M) = {} \<and>
+             even (length p) \<and> distinct p)"
+
+lemma add_alternatingly_precondE:
+   "\<lbrakk>add_alternatingly_precond G M p;
+      \<lbrakk>matching_invar G M; set p \<inter> Vs (matching_abstract M) = {};
+       even (length p); distinct p\<rbrakk> \<Longrightarrow> P\<rbrakk> 
+     \<Longrightarrow> P"
+and  add_alternatingly_precondI:
+   "\<lbrakk>matching_invar G M; set p \<inter> Vs (matching_abstract M) = {};
+       even (length p); distinct p\<rbrakk> 
+    \<Longrightarrow> add_alternatingly_precond G M p"
+  by(auto simp add: add_alternatingly_precond_def)
+end
+
+locale blossom_matching = 
+blossom_matching_spec +
+assumes matching:
+  "\<And> M G. matching_invar G M \<Longrightarrow> graph_matching G (matching_abstract M)"
+  "\<And> G. matching_invar G empty_matching"
+  "matching_abstract empty_matching = {}"
+  "\<And> M G G'. \<lbrakk>matching_invar G M; G \<subseteq> G'\<rbrakk> \<Longrightarrow> matching_invar G' M"
+  "\<And> M G x. \<lbrakk>matching_invar G M; x \<in> Vs (matching_abstract M)\<rbrakk> 
+         \<Longrightarrow>{x, get_partner M x} \<in> matching_abstract M"
+and augment:
+  "\<And> G M p. \<lbrakk>matching_invar G M; graph_augmenting_path G (matching_abstract M) p\<rbrakk> \<Longrightarrow> 
+         matching_invar G (augment M p)"
+  "\<And> G M p. \<lbrakk>matching_invar G M; graph_augmenting_path G (matching_abstract M) p\<rbrakk> \<Longrightarrow> 
+         matching_abstract (augment M p) =  matching_abstract M \<oplus> set (edges_of_path p)"
+and contract:
+  "\<And> G M p new_vert contr. 
+   contract_path_at_matched_precond G M p new_vert contr \<Longrightarrow>
+   matching_invar (quot_graph contr G - {{new_vert}})
+             (contract_path_at_matched M p new_vert)"
+ "\<And> G M p new_vert contr. 
+   contract_path_at_matched_precond G M p new_vert contr \<Longrightarrow>
+   matching_abstract (contract_path_at_matched M p new_vert) 
+    = quot_graph contr (matching_abstract M) - {{new_vert}}"
+and expand: 
+ "\<And> G M old_vert mo new_vert p.
+    expand_path_at_matched_precond G M old_vert mo new_vert p \<Longrightarrow>
+    matching_invar (G - {{old_vert, mo}} \<union> {{new_vert, mo}} 
+                    \<union> {edges_of_path p ! i| i. Suc i < length p \<and> even i}) 
+                   (expand_path_at_matched M p old_vert new_vert)"
+ "\<And> G M old_vert mo new_vert p.
+    expand_path_at_matched_precond G M old_vert mo new_vert p \<Longrightarrow>
+    matching_abstract (expand_path_at_matched M p old_vert new_vert) = 
+    matching_abstract M - {{old_vert, mo}} \<union> {{new_vert, mo}}
+                    \<union> {edges_of_path p ! i| i. Suc i < length p \<and> even i}"
+and add_alternatingly:
+  "\<And> G M p. add_alternatingly_precond G M p \<Longrightarrow>
+            matching_invar (G \<union> {edges_of_path p ! i| i. Suc i < length p \<and> even i})
+            (add_alternatingly M p)"
+ "\<And> G M p. add_alternatingly_precond G M p \<Longrightarrow>
+            matching_abstract (add_alternatingly M p) =
+            matching_abstract M \<union> {edges_of_path p ! i| i. Suc i < length p \<and> even i}"
+
+context 
+  matching_augmentation_spec
+begin
+
+term augment_impl
+
+definition 
+"contract_path_at_matched M p new_vert= 
+  (let u = hd p; v = the (buddy_lookup M u)
+  in (buddy_upd new_vert v (buddy_upd v new_vert 
+         (foldl (\<lambda> M x. buddy_delete x M) M p))))"
+
+definition 
+  "expand_path_at_matched M p old_vert new_vert =
+    (let v = the (buddy_lookup M old_vert);
+         v_rematched = buddy_upd new_vert v (buddy_upd v new_vert (buddy_delete old_vert M))
+     in  augment_impl v_rematched p)"
+
+definition "contract_path_at_matched_precond G M p new_vert contr = 
+            (invar_matching G M \<and> hd p \<in> Vs (\<M> M) \<and> alt_path (\<M> M) p \<and> odd (length p) \<and>
+            distinct p \<and> new_vert \<notin>  Vs (\<M> M) - set p \<and>
+            contr = (\<lambda> x. if x \<in> set p then new_vert else x))"
+
+definition "get_partner M x = the (buddy_lookup M x)"
+
+definition "add_alternatingly = augment_impl"
+
+end
+
+context
+  matching_augmentation
+begin
+
+lemma  get_partner_correct:
+ "\<lbrakk>invar_matching G M; x \<in> Vs (\<M> M)\<rbrakk> \<Longrightarrow>{x, get_partner M x} \<in> \<M> M"
+  using symmetric_buddiesD[of M x] option.collapse[of "buddy_lookup M x"]
+  by(fastforce dest!: invar_matchingD(2) 
+               elim!: vs_member_elim 
+            simp add: get_partner_def \<M>_def' doubleton_eq_iff conj_disj_distribR
+                      ex_disj_distrib  symmetric_buddiesD )  
+
+lemma contract_path_at_matched_effect:
+  assumes "buddy_invar M" "buddy_lookup M (hd p) = Some v"  "buddy_lookup M v = Some (hd p)"
+          "distinct p" "v \<notin> set p" "new_vert \<in> set p \<or> (\<nexists> x. buddy_lookup M new_vert = Some x )"
+  shows "buddy_invar (contract_path_at_matched M p new_vert)"
+        "\<M>_dir (contract_path_at_matched M p new_vert) = 
+         \<M>_dir M - {(x, y) | x y. x \<in> set p \<and> Some y = buddy_lookup M x} 
+                  - {(v, hd p)} \<union> {(v, new_vert),(new_vert, v)}"
+proof-
+  have induct: "buddy_invar (foldl (\<lambda> M x. buddy_delete x M) M p) \<and>
+        buddy_lookup (foldl (\<lambda> M x. buddy_delete x M) M p) = 
+        (\<lambda> x. if x \<in> set p then None else buddy_lookup M x)"
+    using assms(1,4)
+proof(induction p arbitrary: M)
+    case Nil
+    then show ?case 
+      by auto
+  next
+    case (Cons x p)
+    hence distinct_p: "distinct p"
+      by auto
+    note IH = conjunct1[OF Cons(1)[OF _ distinct_p]] conjunct2[OF Cons(1)[OF _ distinct_p]]
+    show ?case 
+    proof(rule, goal_cases)
+      case 1
+      then show ?case 
+        using IH(1) Cons(2) by (auto intro: buddy_map.invar_delete)
+    next
+      case 2 
+      show ?case 
+        unfolding foldl_Cons
+        apply(subst IH(2))
+        using Cons(2)
+        by (auto intro!: buddy_map.invar_delete simp add: Cons.prems buddy_map.map_delete)
+    qed
+  qed
+  hence invar_intermed: "buddy_invar (buddy_upd v new_vert 
+         (foldl (\<lambda> M x. buddy_delete x M) M p))" 
+    using buddy_map.invar_update by force
+  thus "buddy_invar (contract_path_at_matched M p new_vert)" 
+    unfolding contract_path_at_matched_def Let_def assms(2) option.sel
+    by(auto intro!: buddy_map.invar_update)
+  have final_lookup:"buddy_lookup (contract_path_at_matched M p new_vert) = 
+       (\<lambda> x. if x = new_vert then Some v
+             else if x = v then Some new_vert 
+             else if x \<in> set p then None
+             else buddy_lookup M x)"
+    using induct invar_intermed
+    by(auto simp add: contract_path_at_matched_def Let_def buddy_map.map_update assms(2))
+  show "\<M>_dir (contract_path_at_matched M p new_vert) = 
+         \<M>_dir M - {(x, y) | x y. x \<in> set p \<and> Some y = buddy_lookup M x} 
+                  - {(v, hd p)} \<union> {(v, new_vert),(new_vert, v)}"
+    using assms(6) by(auto simp add: \<M>_dir_def' final_lookup if_split[of "\<lambda> x. x = Some _"] assms(3))
+qed
+
+lemma contract_path_at_matched_correct:
+  assumes "invar_matching G M" "hd p \<in> Vs (\<M> M)" "alt_path (\<M> M) p" "odd (length p)"
+          "distinct p" "new_vert \<notin>  Vs (\<M> M) - set p"
+  and contr_def: "contr = (\<lambda> x. if x \<in> set p then new_vert else x)"
+  shows   "invar_matching (quot_graph contr G - {{new_vert}})
+             (contract_path_at_matched M p new_vert)" (is ?th1)
+          "\<M> (contract_path_at_matched M p new_vert) = quot_graph contr (\<M> M) - {{new_vert}}" (is ?th2)
+proof-
+  note invar_matching_here = invar_matchingD[OF assms(1)]
+
+  obtain v where v: "buddy_lookup M (hd p) = Some v" "buddy_lookup M v = Some (hd p)"
+    using assms(2) invar_matching_here(2) 
+    by(auto elim!: symmetric_buddiesE simp add: \<M>_def' vs_member) 
+
+  hence hdp_v_in_M:"{hd p, v} \<in> \<M> M" and  hdp_v_in_M':"{v, hd p} \<in> \<M> M"
+    by(auto simp add: \<M>_def')
+  have dblton_M: "dblton_graph (\<M> M)" 
+    by (simp add: invar_matching_here(3) no_self_loop_buddy_dblton_graph)
+  have matching_M:"matching (\<M> M)"
+    by (simp add: invar_matching_here(4))
+  have p_split_off_tl: "p = hd p # tl p" 
+    by (metis assms(4) even_zero list.exhaust_sel list.size(3))
+
+  have rev_alt_path: "rev_alt_path (\<M> M) (tl p)" 
+    by (simp add: alt_path_tl_rev_alt_path assms(3))
+
+  have v_neq_hd_p:"v \<noteq> hd p"
+    using invar_matching_here(3) no_self_loop_buddyE v(2) by blast
+  have even_tl: "even (length (tl p))"
+    by (simp add: assms(4))
+  note path_edge_cases = matching_edge_rev_alt_path_cases[OF rev_alt_path _ dblton_M matching_M]
+
+  have v_in_set_p:"v \<notin> set p" 
+  proof(rule ccontr, goal_cases)
+    case 1
+    hence v_tl: "v \<in> set (tl p)" and "length p \<ge> 3"
+      using v_neq_hd_p assms(4) by(all \<open>cases p rule: list_cases4\<close>) auto
+    hence tl_longer_1:"1 < length (tl p)" by auto
+    obtain e where e: "e \<in> set (edges_of_path (tl p))" "v \<in> e" "e \<in> \<M> M"
+      using in_rev_alt_path_part_of_matching[OF rev_alt_path v_tl even_tl tl_longer_1] by auto
+    show ?case
+    proof(cases rule: path_edge_cases[OF e(3)])
+      case (1 u' v' i)
+      hence "e = {hd p, v}"
+        using e(2,3)  hdp_v_in_M  matching_unique_match[OF matching_M] by simp
+      hence "hd p \<in> set (tl p)" 
+        using  e(1) edge_not_in_edges_in_path[of "hd p" "tl p"] by auto
+      hence  "\<not> distinct p" 
+        by(cases p) auto
+      then show ?thesis 
+        using assms(5) by simp
+    next
+      case (2 u v)
+      then show ?thesis 
+        using even_tl by fastforce
+    next
+      case 3
+      then show ?thesis
+        using e(2) v_tl by auto
+    qed
+  qed
+
+  have new_vert_in_p_or_not_buddy:"new_vert \<in> set p \<or> (\<nexists>x. buddy_lookup M new_vert = Some x)" 
+    using assms(6) by (auto simp add: \<M>_def')
+
+  note contract_path_at_matched_effect =
+       contract_path_at_matched_effect[OF invar_matching_here(1) v assms(5)
+                                            v_in_set_p new_vert_in_p_or_not_buddy]
+
+  have lookup_and_p_heler1:
+  "\<lbrakk>va \<in> set p; Some u = buddy_lookup M va; va \<noteq> v; u \<noteq> v\<rbrakk> \<Longrightarrow> u \<in> set p" for va u 
+  proof(goal_cases)
+    case 1
+    hence v_tl: "va \<in> set (tl p)"  
+      using v(1) by(cases p) auto
+    hence tl_longer_1:"1 < length (tl p)"
+      using even_tl by(cases p rule: list_cases4) auto
+    from 1 have uva_in_M: "{u, va} \<in> \<M> M" 
+      by(force simp add: \<M>_def' doubleton_eq_iff)
+    moreover obtain e where e: "e \<in> set (edges_of_path (tl p))" "va \<in> e" "e \<in> \<M> M"
+      using in_rev_alt_path_part_of_matching[OF rev_alt_path v_tl even_tl tl_longer_1] by auto
+    ultimately have "u \<in> set (tl p)"
+      using matching_unique_match[OF matching_M, of va e "{u, va}", simplified]
+      by(auto intro!: v_in_edge_in_path[of u va "tl p"]) 
+    thus ?case
+      by(cases p) auto
+  qed
+
+  have hd_p_in_p:"hd p \<in> set p" 
+    using p_split_off_tl by(cases p) auto
+
+  have lookup_and_p_heler2:
+  "\<lbrakk>u \<in> set p; Some u = buddy_lookup M va; va \<noteq> v; u \<noteq> v\<rbrakk> \<Longrightarrow> va \<in> set p" for va u 
+    using invar_matching_here(2) symmetric_buddiesD[of M u va] lookup_and_p_heler1[of u va] by auto
+
+  have symm_buddies_after:
+     "symmetric_buddies (contract_path_at_matched M p new_vert)"
+      using invar_matching_here(2) v(2) v_in_set_p hd_p_in_p
+      by(auto elim!: symmetric_digraphE
+             intro!: symmetric_digraphI 
+           simp add: symmetric_digraph_iff_symmetric_buddies
+                     contract_path_at_matched_effect(2)
+              symmetric_buddiesD[OF invar_matching_here(2), simplified eq_commute[of _ "Some _"]]
+               dest: lookup_and_p_heler1 lookup_and_p_heler2)
+
+    have v_neq_new_vert: "v \<noteq> new_vert"
+      using new_vert_in_p_or_not_buddy v(2) v_in_set_p by blast
+
+    have no_self_loop_buddy_after: "no_self_loop_buddy (contract_path_at_matched M p new_vert)"
+      using v_neq_new_vert invar_matching_here(3) 
+      by(auto intro!: no_self_loop_buddyI
+            simp add: no_self_loop_buddy_and_\<M>_dir contract_path_at_matched_effect(2))
+
+    have M_contract_is_UD:"\<M> (contract_path_at_matched M p new_vert) = 
+          \<M> M - {{x, y} |x y. x \<in> set p \<and> Some y = buddy_lookup M x} \<union>
+        {{v, new_vert}}"
+      unfolding \<M>_\<M>_dir_UD contract_path_at_matched_effect(2)
+    proof(rule, all\<open>rule\<close>, goal_cases)
+      case (1 e)
+      then obtain u' v'  where
+        "(u', v') \<in> \<M>_dir M - ({(x, y) |x y. x \<in> set p \<and> Some y = buddy_lookup M x} \<union> {(v, hd p)})
+         \<union> {(v, new_vert), (new_vert, v)}"
+           "e = {u', v'}"
+        unfolding UD_def by blast
+      then show ?case 
+      proof(elim UnE, goal_cases)
+        case 1
+        note one = this
+        show ?case 
+        proof(rule UnI1, rule DiffI, goal_cases)
+          case 1
+          then show ?case 
+            using one by (simp add: in_UDI)
+        next
+          case 2
+          show ?case 
+          proof(rule ccontr, goal_cases)
+            case 1
+            hence "(u', v') \<in> {(x, y) |x y. x \<in> set p \<and> Some y = buddy_lookup M x}"
+              using v(2) v_in_set_p invar_matching_here(2) one(2)
+              by (auto elim!: symmetric_buddiesE 
+                    simp add: one(1) doubleton_eq_iff
+                              symmetric_buddiesD[OF invar_matching_here(2),
+                                  simplified eq_commute[of _ "Some _"]]
+                       intro: lookup_and_p_heler1
+                        dest: lookup_and_p_heler1)
+            then show ?case
+              using one(2) by force
+          qed 
+        qed
+      qed auto
+    next
+      case (2 e)
+      then show ?case 
+      proof(elim UnE, goal_cases)
+        case 1
+        moreover then obtain u' v' where "e = {u', v'}" "(u',v') \<in> \<M>_dir M"
+          by (auto simp add: UD_def)
+        ultimately show ?case
+          using hd_p_in_p v(1)
+          by(fastforce intro!: in_UDI[of u' v'])
+    qed (auto simp add: UD_def)
+  qed
+
+  have x_buddies_helper:
+      "{{x, y} |x y. x \<in> set p \<and> Some y = buddy_lookup M x} = 
+        insert {hd p, v} {edges_of_path p ! i | i. Suc i < length p \<and> odd i}"
+  proof-
+    have "{{x, y} |x y. x \<in> set p \<and> Some y = buddy_lookup M x} = 
+         insert {hd p, v} {e| e. e \<in> \<M> M  \<and> e \<inter> set (tl p) \<noteq> {}}"
+       unfolding  \<M>_def'
+    proof(subst p_split_off_tl, rule, goal_cases)
+      case 1
+      then show ?case 
+        using v invar_matching_here(2) by force
+    next
+      case 2
+      then show ?case
+      using invar_matching_here(2) v
+      by(fastforce elim!: symmetric_buddiesE 
+                simp add: doubleton_eq_iff symmetric_buddiesD[OF invar_matching_here(2),
+                          simplified eq_commute[of _ "Some _"]])
+  qed
+    moreover have "{e| e. e \<in> \<M> M  \<and> e \<inter> set (tl p) \<noteq> {}} = 
+               {edges_of_path (tl p) ! i | i. Suc i < length (tl p) \<and> even i}" 
+      using even_tl matched_verts_in_rev_alt_path_path_edges matching_M rev_alt_path by blast
+    moreover have "... = {edges_of_path p ! i | i. Suc i < length p \<and> odd i}" 
+      using assms(4) less_Suc_eq_0_disj 
+      by(cases p rule: list_cases3)(auto intro:  exI[of _ "Suc _"])
+    ultimately show ?thesis 
+      by simp
+  qed
+    
+  have set_2diff_distr: "A - B - C = A - (B \<union> C)" for A B C by auto
+
+  have set_minus_absorb: "A - B = A - (A \<inter> B)" for A B by auto
+
+  have UD_helper:
+   "UD ({(x, y) |x y. x \<in> set p \<and> Some y = buddy_lookup M x} \<union> {(v, hd p)}) = 
+     insert {hd p, v} {edges_of_path p ! i |i. Suc i < length p \<and> odd i}"
+    using hd_p_in_p v(1)
+    unfolding x_buddies_helper[symmetric]
+    by(fastforce simp add: UD_def)
+  have edges_of_p_split_off_v: "edges_of_path (v # p) = {v,hd p} # edges_of_path p" 
+    using hd_p_in_p by(cases p) auto
+  have SD_here: 
+      "symmetric_digraph ({(x, y) |x y. x \<in> set p \<and> Some y = buddy_lookup M x} \<union> {(v, hd p)})"
+   using lookup_and_p_heler1 v_in_set_p v
+   by(auto elim!: symmetric_buddiesE
+          intro!: symmetric_digraphI
+        simp add: hd_p_in_p  
+                  symmetric_buddiesD[OF invar_matching_here(2), simplified eq_commute[of _ "Some _"]]
+           dest:lookup_and_p_heler1)
+  have Suc_i_less_p_is:"Suc i < length p \<longleftrightarrow> i < length (edges_of_path p)" for i p
+    using assms(4) by(cases p) (auto simp add: edges_of_path_length)
+  have rev_alt_v:"rev_alt_path (\<M> M) (v # p)"
+    by(auto simp add: alt_list_step assms(3) edges_of_p_split_off_v hdp_v_in_M')
+
+  show th2: ?th2
+      unfolding \<M>_\<M>_dir_UD contract_path_at_matched_effect(2) UD_union_hom
+                set_2diff_distr
+      unfolding UD_diff_hom[OF SD_here]
+      unfolding UD_helper \<M>_\<M>_dir_UD[symmetric] UD_of_swapped_pairs
+      unfolding alt_path_matching_quot[OF matching_M hdp_v_in_M' assms(3,4)
+                         dblton_M assms(5,6) contr_def]
+    proof(rule arg_cong2[where f = Set.union], subst (2) set_minus_absorb,
+          subst rev_alt_path_intersected_with_matching[OF matching_M rev_alt_v], goal_cases)
+      case 1
+      thus ?case
+      unfolding edges_of_p_split_off_v Suc_i_less_p_is
+      using nth_Cons_0[of "{v, hd p}" "edges_of_path p"]
+            nth_Cons_Suc[of "{v, hd p}" "edges_of_path p"] 
+      by (fastforce simp add: less_Suc_eq_0_disj insert_commute)+
+  qed auto
+
+  have graph_matching_after:
+    "graph_matching (quot_graph contr G - {{new_vert}}) (\<M> (contract_path_at_matched M p new_vert))"
+    using invar_matching_here(4) assms(3,4,5,6)  dblton_M
+    by(unfold th2, intro alt_path_contract_matching[OF _ hdp_v_in_M']) (auto simp add: contr_def)
+  have finite_after: "finite (\<M> (contract_path_at_matched M p new_vert))"
+    by (simp add: M_contract_is_UD invar_matching_here(5))
+
+  show ?th1
+   by(intro invar_matchingI symm_buddies_after contract_path_at_matched_effect(1)
+            no_self_loop_buddy_after graph_matching_after finite_after)
+qed
+
+lemma expand_path_at_matched_effect:
+  assumes "buddy_invar M" "distinct p" "even (length p)" "set p \<inter> dVs (\<M>_dir M) = {}"
+          "buddy_lookup M old_vert = Some ovn" 
+           "ovn \<notin> set p" "new_vert \<notin> set p"
+        shows"buddy_invar (expand_path_at_matched M p old_vert new_vert)"
+   and  "\<M>_dir (expand_path_at_matched M p old_vert new_vert) =
+     \<M>_dir M 
+   - {(x, y) | x y. x \<in> {old_vert, new_vert,ovn} \<and> buddy_lookup M x = Some y} 
+   \<union> {(new_vert, ovn), (ovn, new_vert)} - {(u, v) |u v. u \<in> set p \<and> buddy_lookup M u = Some v} \<union>
+  \<Union> {{(u, v), (v, u)}| u v i. u = p ! i \<and> v = p ! (i + 1) \<and> i + 1 < length p \<and> even i}"
+ (is ?ths)
+proof-
+  define v_rematched where 
+      "v_rematched = buddy_upd new_vert (the (buddy_lookup M old_vert))
+                 (buddy_upd (the (buddy_lookup M old_vert)) new_vert (buddy_delete old_vert M))"
+  have intermed: "buddy_invar v_rematched"
+   "\<M>_dir v_rematched = \<M>_dir M 
+   - {(x, y) | x y. x \<in> {old_vert, new_vert,ovn} \<and> buddy_lookup M x = Some y} 
+   \<union> {(new_vert, ovn), (ovn, new_vert)}"
+   by(auto intro!: buddy_map.invar_update buddy_map.invar_delete 
+             simp add: v_rematched_def \<M>_dir_def' assms(1)  if_split[of "\<lambda> x. x = Some _"] assms(5)
+             | subst (asm) buddy_map.map_update buddy_map.map_delete
+             | subst  buddy_map.map_update buddy_map.map_delete)+
+  have u_in_p_same:"u \<in> set p \<Longrightarrow> buddy_lookup v_rematched u = buddy_lookup M u" for u
+  proof( goal_cases)
+    case 1
+    have "(u, v) \<in> \<M>_dir v_rematched \<longleftrightarrow> (u, v) \<in> \<M>_dir M" for v
+        using 1 assms(7) assms(4) by(auto simp add: intermed(2) assms(5,6) assms(7))
+      then show ?case 
+        using 1 assms(4)
+        by(cases "buddy_lookup v_rematched u")(fastforce simp add: \<M>_dir_def')+ 
+    qed
+    moreover have exp:"expand_path_at_matched M p old_vert new_vert = 
+                   augment_impl v_rematched p"
+      by(auto simp add: expand_path_at_matched_def v_rematched_def Let_def)
+    thus "buddy_invar (expand_path_at_matched M p old_vert new_vert)"
+      using intermed augment_impl_effect(1)[OF intermed(1) assms(2,3)]
+      by simp
+    show ?ths
+      unfolding exp intermed augment_impl_effect(2)[OF intermed(1) assms(2,3)]
+      by(auto simp add: u_in_p_same)
+  qed
+
+lemma extend_graph: 
+ "\<lbrakk>invar_matching G M; G \<subseteq> G'\<rbrakk> \<Longrightarrow> invar_matching G' M"
+  by(auto elim!: invar_matchingE intro!: invar_matchingI)
+
+lemma expand_path_at_matched_correct:
+  assumes "invar_matching G M" "{old_vert, mo} \<in> \<M> M" "new_vert \<notin> Vs (\<M> M) - {old_vert}"
+          "new_vert \<notin> set p" "set p \<inter> Vs (\<M> M) = {}" "even (length p)" "distinct p"
+ and new_matching_def: "M' = \<M> M - {{old_vert, mo}} \<union> {{new_vert, mo}}
+         \<union> {edges_of_path p ! i| i. Suc i < length p \<and> even i}"
+shows "invar_matching (G - {{old_vert, mo}} \<union> {{new_vert, mo}} 
+                       \<union> {edges_of_path p ! i| i. Suc i < length p \<and> even i}) 
+           (expand_path_at_matched M p old_vert new_vert)" (is ?th1)
+      "\<M> (expand_path_at_matched M p old_vert new_vert) = M'" (is ?th2)
+proof-
+
+  note invar_matching_here = invar_matchingD[OF assms(1)]
+
+  have effect_precond1: "set p \<inter> dVs (\<M>_dir M) = {}"
+    using assms(5) by(auto elim!: in_dVsE(1) simp add: \<M>_def' \<M>_dir_def' Vs_def)
+  have effect_precond2: "buddy_lookup M old_vert = Some mo"
+    using assms(2)  invar_matching_here(2) 
+    by(auto simp add: \<M>_def' symmetric_buddiesD doubleton_eq_iff)
+  have effect_precond3: "mo \<notin> set p" "new_vert \<notin> set p"
+    using assms(2,3,4,5)
+    invar_matching_here(2) 
+    by(auto dest: edges_are_Vs_2 
+        simp add: \<M>_def' symmetric_buddiesD doubleton_eq_iff vs_member edges_are_Vs_2) blast+
+  note effect_here = expand_path_at_matched_effect[OF 
+          invar_matching_here(1) assms(7,6) effect_precond1 effect_precond2 effect_precond3]
+
+  have lookup1: "buddy_lookup M v = Some new_vert \<Longrightarrow> v = mo"
+                "buddy_lookup M v = Some mo \<Longrightarrow> v = old_vert"for v
+    using assms(2,3) effect_precond2 symmetric_buddiesD[OF invar_matching_here(2)] effect_precond2
+    by(auto simp add: vs_member \<M>_def' doubleton_eq_iff)+
+    
+
+  show th2: ?th2
+    unfolding \<M>_\<M>_dir_UD effect_here UD_union_hom new_matching_def
+  proof(rule arg_cong2[where f = Set.union], goal_cases)
+    case 1
+    then show ?case 
+    proof(subst (2) Diff_triv, goal_cases)
+      case 1
+      then show ?case 
+        using effect_precond1
+        by (auto simp add: effect_precond3)
+    next
+      case 2
+      show ?case
+        unfolding UD_union_hom
+      proof(rule arg_cong2[where f = Set.union], goal_cases)
+        case 1
+        show ?case 
+        proof(subst UD_diff_hom, goal_cases)
+          case 1
+          then show ?case 
+            using invar_matching_here(2) effect_precond2  assms(3)
+            by(auto intro!: symmetric_digraphI simp add: symmetric_buddiesD \<M>_def')
+              (simp add: symmetric_buddiesD[of M old_vert, symmetric]
+                symmetric_buddiesD[of M old_vert mo, symmetric])+
+        next
+          case 2
+          then show ?case 
+            using assms(3) invar_matching_here(2) 
+            by (intro arg_cong2[where f = "(-)"])
+               (auto intro!: exI[of "\<lambda> u. \<exists> v. _ v u", of _ old_vert] 
+                   simp add: UD_def \<M>_def' effect_precond2 symmetric_buddiesD lookup1 vs_member 
+                       dest: lookup1)
+        qed
+      next
+        case 2
+        then show ?case 
+          by (simp add: UD_of_swapped_pairs)
+      qed
+    qed
+  next
+    case 2
+    then show ?case 
+      using edges_of_path_index
+      by(auto simp add: UD_def) blast
+  qed
+
+  have symmetric_buddies_after:
+      "symmetric_buddies (expand_path_at_matched M p old_vert new_vert)"
+    unfolding symmetric_digraph_iff_symmetric_buddies effect_here(2)
+  proof(rule symmetric_union_pres, goal_cases)
+    case 1
+    then show ?case 
+    proof(rule symmetric_diff_pres, goal_cases)
+      case 1
+      then show ?case 
+        using invar_matching_here(2) effect_precond2
+              symmetric_buddiesD[of M mo old_vert, OF invar_matching_here(2)] 
+        by(auto elim!: symmetric_digraphE 
+               intro!: symmetric_digraphI
+             simp add: symmetric_digraph_iff_symmetric_buddies  
+                       lookup1(1) 
+                       symmetric_buddiesD[OF invar_matching_here(2), of old_vert, symmetric]
+                       symmetric_buddiesD[OF invar_matching_here(2), of old_vert mo, symmetric]
+                       symmetric_buddiesD[of M _ new_vert, OF invar_matching_here(2)], auto?)
+    next
+      case 2
+      then show ?case 
+        using assms(5) edges_are_Vs_2
+        by(auto intro!: symmetric_digraphI simp add: \<M>_def')blast+
+    qed
+  next
+    case 2
+    then show ?case 
+      by(auto intro!: symmetric_digraphI)
+  qed
+
+  have no_self_loop_buddy_after: 
+     "no_self_loop_buddy (expand_path_at_matched M p old_vert new_vert)"
+    using effect_precond2 invar_matching_here(3) lookup1(1)
+    by(auto elim!: no_self_loop_buddyE 
+         simp add: no_self_loop_buddy_and_\<M>_dir effect_here(2) assms(7) nth_eq_iff_index_eq
+            intro: no_self_loop_buddyE[OF invar_matching_here(3)]) 
+
+  have matching_after:
+   "graph_matching (G - {{old_vert, mo}} \<union> {{new_vert, mo}} 
+                    \<union> {edges_of_path p ! i |i. Suc i < length p \<and> even i})
+     (\<M> (expand_path_at_matched M p old_vert new_vert))"
+  proof(rule, goal_cases)
+    case 1
+    then show ?case 
+      unfolding th2 new_matching_def
+    proof(rule matching_vertex_disj_union, goal_cases)
+      case 1
+      then show ?case 
+      using assms(2,3) invar_matching_here(4)
+      by(auto intro!: matchingI elim!: matchingE)
+    next
+      case 2
+      then show ?case
+        by(auto intro!: even_edges_of_distinct_path_are_matching simp add: assms(7))
+    next
+      case 3
+      have i_smp:"i < length p - 1 \<longleftrightarrow> Suc i < length p" for i
+        by (simp add: less_diff_conv)
+      show ?case 
+        using   assms(5,6) effect_precond3
+        by (auto elim!: vs_member_elim simp add: verts_of_even_eges[of p, simplified i_smp])
+    qed
+  next
+    case 2
+    then show ?case 
+      using invar_matching_here(4)
+      by(auto simp add: th2 new_matching_def)
+  qed
+
+  have finite_after: "finite (\<M> (expand_path_at_matched M p old_vert new_vert))" 
+    by(auto intro!: finite_subset[of _ "set (edges_of_path p)"] 
+          simp add: th2 new_matching_def invar_matching_here(5) edges_of_path_length)
+ 
+  show ?th1
+  proof(rule invar_matchingI, goal_cases)
+    case 1
+    then show ?case 
+      by (simp add: effect_here(1))
+  next
+    case 2
+    then show ?case 
+      using symmetric_buddies_after by simp
+  next
+    case 3
+    then show ?case
+      using no_self_loop_buddy_after by simp
+  next
+    case 4
+    then show ?case 
+      using matching_after by simp
+  next
+    case 5
+    then show ?case 
+      using finite_after by simp
+  qed
+qed
+
+lemma add_alternatingly_correct:
+  assumes "invar_matching G M"  "set p \<inter> Vs (\<M> M) = {}" "even (length p)" "distinct p"
+ and new_matching_def: "M' = \<M> M 
+         \<union> {edges_of_path p ! i| i. Suc i < length p \<and> even i}"
+shows "invar_matching (G \<union> {edges_of_path p ! i| i. Suc i < length p \<and> even i}) 
+           (add_alternatingly M p)" (is ?th1)
+      "\<M> (add_alternatingly M p) = M'" (is ?th2)
+proof-
+
+  note invar_matching_here = invar_matchingD[OF assms(1)]
+
+  note augment_impl_effect_here = augment_impl_effect[OF invar_matching_here(1) assms(4,3)]
+
+  have M_dir_with_p: "\<lbrakk>(u, v) \<in> \<M>_dir M; v \<in> set p \<or> u \<in> set p\<rbrakk> \<Longrightarrow> False" for u v
+    using assms(2) by(auto simp add: \<M>_\<M>_dir_UD Vs_dVs_UD)
+
+
+  show th2: ?th2
+    unfolding \<M>_\<M>_dir_UD add_alternatingly_def 
+              augment_impl_effect_here(2) UD_union_hom new_matching_def
+  proof(rule arg_cong2[where f = Set.union], goal_cases)
+    case 1
+    then show ?case 
+    proof(subst Diff_triv, goal_cases)
+      case 1
+      then show ?case
+        by (auto dest: M_dir_with_p)
+    next
+    qed simp
+  next
+    case 2
+    then show ?case 
+      using edges_of_path_index
+      by(auto simp add: UD_def) blast
+  qed
+
+  have symmetric_buddies_after:
+      "symmetric_buddies (add_alternatingly M p)"
+    unfolding symmetric_digraph_iff_symmetric_buddies add_alternatingly_def 
+              augment_impl_effect_here(2)
+  proof(rule symmetric_union_pres, goal_cases)
+    case 1
+    then show ?case 
+    proof(rule symmetric_diff_pres, goal_cases)
+      case 1
+      then show ?case 
+        using invar_matching_here(2) symmetric_digraph_iff_symmetric_buddies by blast
+    next
+      case 2
+      then show ?case 
+        using assms(2) edges_are_Vs_2
+        by(auto intro!: symmetric_digraphI simp add: \<M>_def')blast+
+    qed
+  next
+    case 2
+    then show ?case 
+      by(auto intro!: symmetric_digraphI)
+  qed
+
+  have no_self_loop_buddy_after: 
+     "no_self_loop_buddy (add_alternatingly M p)"
+    using invar_matching_here(3) 
+    by(auto elim!: no_self_loop_buddyE 
+         simp add: no_self_loop_buddy_and_\<M>_dir  nth_eq_iff_index_eq 
+                   add_alternatingly_def augment_impl_effect_here(2) assms(4)
+            intro: no_self_loop_buddyE[OF invar_matching_here(3)]) 
+
+  have matching_after:
+   "graph_matching (G \<union> {edges_of_path p ! i |i. Suc i < length p \<and> even i})
+     (\<M> (add_alternatingly M p))"
+  proof(rule, goal_cases)
+    case 1
+    then show ?case 
+      unfolding th2 new_matching_def
+    proof(rule matching_vertex_disj_union, goal_cases)
+      case 1
+      then show ?case 
+      using assms(2,3) invar_matching_here(4)
+      by(auto intro!: matchingI elim!: matchingE)
+    next
+      case 2
+      then show ?case
+        by(auto intro!: even_edges_of_distinct_path_are_matching simp add: assms(4))
+    next
+      case 3
+      have i_smp:"i < length p - 1 \<longleftrightarrow> Suc i < length p" for i
+        by (simp add: less_diff_conv)
+      show ?case 
+        using  assms(2,3) 
+        by (auto elim!: vs_member_elim simp add: verts_of_even_eges[of p, simplified i_smp])
+    qed
+  next
+    case 2
+    then show ?case 
+      using invar_matching_here(4)
+      by(auto simp add: th2 new_matching_def)
+  qed
+
+  have finite_after: "finite (\<M> (add_alternatingly M p))" 
+    by(auto intro!: finite_subset[of _ "set (edges_of_path p)"] 
+          simp add: th2 new_matching_def invar_matching_here(5) edges_of_path_length)
+ 
+  show ?th1
+  proof(rule invar_matchingI, goal_cases)
+    case 1
+    then show ?case 
+      by (simp add: add_alternatingly_def augment_impl_effect_here(1))
+  next
+    case 2
+    then show ?case 
+      using symmetric_buddies_after by simp
+  next
+    case 3
+    then show ?case
+      using no_self_loop_buddy_after by simp
+  next
+    case 4
+    then show ?case 
+      using matching_after by simp
+  next
+    case 5
+    then show ?case 
+      using finite_after by simp
+  qed
+qed
+
+
+
+interpretation blossom_matching_spec_here:
+  blossom_matching_spec 
+  where empty_matching = empty_matching
+  and matching_invar = invar_matching
+  and augment =augment_impl
+  and matching_abstract = \<M>
+  and contract_path_at_matched = contract_path_at_matched
+  and expand_path_at_matched = expand_path_at_matched
+  done
+
+interpretation blossom_matching_here:
+  blossom_matching 
+  where empty_matching = empty_matching
+  and matching_invar = invar_matching
+  and augment =augment_impl
+  and matching_abstract = \<M>
+  and contract_path_at_matched = contract_path_at_matched
+  and expand_path_at_matched = expand_path_at_matched
+  and get_partner = get_partner
+  and add_alternatingly = add_alternatingly
+proof(rule blossom_matching.intro, goal_cases)
+  case (1 M G)
+  then show ?case
+    using invar_matchingD(4) by auto
+next
+  case (2 G)
+  then show ?case 
+    by (simp add: empty_matching_props')
+next                                          
+  case 3
+  then show ?case 
+   by (simp add: empty_matching_props')
+next
+  case (4 M G G')
+  thus ?case
+    using extend_graph by blast
+next
+  case (5 x M G)
+  thus ?case
+    using get_partner_correct by blast
+next
+  case (6 G M p)
+  then show ?case 
+    by (simp add: augmentation_correct(1))
+next
+  case (7 G M p)
+  then show ?case 
+    by (simp add: augmentation_correct(2))
+next
+  case (8 G M p new_vert contr)
+  then show ?case 
+    by(elim blossom_matching_spec_here.contract_path_at_matched_precondE,
+       intro contract_path_at_matched_correct)
+next
+  case (9 G M p new_vert contr)
+  then show ?case 
+  by(elim blossom_matching_spec_here.contract_path_at_matched_precondE,
+       intro contract_path_at_matched_correct)
+next
+  case (10 G M old_vert mo new_vert p)
+  thus ?case
+    by(elim blossom_matching_spec_here.expand_path_at_matched_precondE, 
+       intro expand_path_at_matched_correct) 
+       auto
+next
+  case (11 G M old_vert mo new_vert p)
+  thus ?case
+    by(elim blossom_matching_spec_here.expand_path_at_matched_precondE, 
+       intro expand_path_at_matched_correct) 
+       auto 
+next
+  case (12 G M p)
+  thus ?case
+    by(elim blossom_matching_spec_here.add_alternatingly_precondE,
+       intro add_alternatingly_correct)
+       auto
+next
+  case (13 G M p)
+  thus ?case
+    by(elim blossom_matching_spec_here.add_alternatingly_precondE,
+       intro add_alternatingly_correct)
+       auto
+qed
+
+lemmas blossom_matching_spec_satisfied = blossom_matching_here.blossom_matching_axioms
+
+end
+
+thm matching_augmentation.blossom_matching_spec_satisfied
+end
